lib/smack/SmackSrcNamesMapper.cpp
@@ -1,0 +1,107 @@
+//
+// This file is distributed under the MIT License. See LICENSE for details.
+//
+#define DEBUG_TYPE "smack-inst-gen"
+#include "smack/SmackSrcNamesMapper.h"
+#include "smack/Debug.h"
+#include "smack/Naming.h"
+#include "smack/SmackOptions.h"
+#include "llvm/IR/Value.h"
+#include "llvm/Analysis/LoopInfo.h"
+#include "llvm/IR/DebugInfo.h"
+#include "llvm/IR/GetElementPtrTypeIterator.h"
+#include "llvm/IR/InstVisitor.h"
+#include "llvm/Support/GraphWriter.h"
+#include <sstream>
+
+#include "llvm/Support/raw_ostream.h"
+#include <iostream>
+
+#include "smack/SmackWarnings.h"
+
+namespace smack {
+
+using llvm::errs;
+using namespace llvm;
+
+// const bool SHOW_ORIG = false;
+
+// #define ORIG(ins)                                                              \
+//   if (SHOW_ORIG)                                                               \
+//   emit(Stmt::comment(i2s(ins)))
+
+// Regex VAR_DECL("^[[:space:]]*var[[:space:]]+([[:alpha:]_.$#'`~^\\?][[:alnum:]_."
+//                "$#'`~^\\?]*):.*;");
+
+// // Procedures whose return value should not be marked as external
+// Regex EXTERNAL_PROC_IGNORE("^(malloc|__VERIFIER_nondet)$");
+
+
+
+
+
+void SmackSrcNamesMapper::visitBasicBlock(llvm::BasicBlock &bb) {
+  SDEBUG(errs() << "visitBasicBlock" << "\n");
+  nextInst = bb.begin();
+  //emit(Stmt::symbheap(se->getCurrSH()));
+  auto *F = bb.getParent();
+  if (&bb == &F->getEntryBlock()) {
+    for (auto &I : bb.getInstList()) {
+      if (llvm::isa<llvm::DbgInfoIntrinsic>(I))
+        continue;
+      if (I.getDebugLoc()) {
+        break;
+      }
+    }
+  }
+}
+
+void SmackSrcNamesMapper::visitInstruction(llvm::Instruction &inst) {
+  SDEBUG(errs() << "Instruction not handled: " << inst << "\n");
+}
+
+
+
+void SmackSrcNamesMapper::visitDbgValueInst(llvm::DbgValueInst &dvi) {
+  SDEBUG(errs() << "visitDbgValue" << "\n");
+  /*se->executeOther();
+  emit(Stmt::symbheap(se->getCurrSH()));*/
+  if (SmackOptions::SourceLocSymbols) {
+    const llvm::Value *V = dvi.getValue();
+    const llvm::DILocalVariable *var = dvi.getVariable();
+    errs() << "Var name: " << var->getName()  << "\n";  
+    if (naming->hasName(*V)) {
+        errs() << "Has Name: " << naming->get(*V) << "\n";
+        if(this->mappedNames.find(V) != this->mappedNames.end()){
+            errs() << "Repeated: " << *V << "\n";
+        }
+        this->mappedNames[V] = naming->get(*V);
+        this->sourceNames[naming->get(*V)] = V;
+    }
+    // if (V && !V->getType()->isPointerTy() && !llvm::isa<ConstantInt>(V)) {
+    if (V && !V->getType()->isPointerTy()) {
+      // if (currBlock->begin() != currBlock->end()
+      //&& currBlock->getStatements().back()->getKind() == Stmt::ASSUME) {
+      //    && isSourceLoc(currBlock->getStatements().back())) {
+      // assert(&*currInst == &dvi && "Current Instruction mismatch!");
+      
+      auto currInst = std::prev(nextInst);
+      if (currInst != dvi.getParent()->begin()) {
+        const Instruction &pi = *std::prev(currInst);
+        V = V->stripPointerCastsAndAliases();
+        if (!llvm::isa<const PHINode>(&pi) &&
+            V == llvm::dyn_cast<const Value>(&pi)){
+
+            }
+      }
+      Function *F = dvi.getFunction();
+      for (auto &arg : F->args()) {
+        if (&arg == V && var->getScope() == F->getMetadata("dbg")) {
+          break;
+        }
+      }
+    }
+  }
+} 
+
+} // namespace smack
