testcases/printtest/exec_IR.ll
@@ -1,28 +1,19 @@
-; ModuleID = '/home/clexma/Desktop/Disk_D/Tools/SESL/SESL/build/b-qbn7no6i.bc'
+; ModuleID = '/home/clexma/Desktop/Disk_D/Tools/SESL/SESL/build/b-8xp6myxi.bc'
 source_filename = "llvm-link"
 target datalayout = "e-m:e-p270:32:32-p271:32:32-p272:64:64-i64:64-f80:128-n8:16:32:64-S128"
 target triple = "x86_64-pc-linux-gnu"
 
 ; Function Attrs: noinline nounwind uwtable
 define dso_local i32 @main() #0 !dbg !10 {
-  call void @llvm.dbg.value(metadata i32 5, metadata !13, metadata !DIExpression()), !dbg !14, !verifier.code !15
-  %1 = sext i32 5 to i64, !dbg !16, !verifier.code !15
-  %2 = mul i64 %1, 4, !dbg !17, !verifier.code !15
-  %3 = call noalias i8* @malloc(i64 %2) #3, !dbg !18, !verifier.code !15
-  %4 = bitcast i8* %3 to i32*, !dbg !19, !verifier.code !15
-  call void @llvm.dbg.value(metadata i32* %4, metadata !20, metadata !DIExpression()), !dbg !14, !verifier.code !15
-  %5 = add nsw i32 5, -1, !dbg !21, !verifier.code !15
-  %6 = getelementptr inbounds i32, i32* %4, i64 1, !dbg !22, !verifier.code !15
-  store i32 %5, i32* %6, align 4, !dbg !23, !verifier.code !15
-  %7 = getelementptr inbounds i32, i32* %4, i64 1, !dbg !24, !verifier.code !15
-  %8 = load i32, i32* %7, align 4, !dbg !25, !verifier.code !15
-  %9 = add nsw i32 %8, -1, !dbg !26, !verifier.code !15
-  call void @llvm.dbg.value(metadata i32 %9, metadata !27, metadata !DIExpression()), !dbg !14, !verifier.code !15
-  %10 = bitcast i32* %4 to i8*, !dbg !28, !verifier.code !15
-  call void @free(i8* %10) #3, !dbg !29, !verifier.code !15
-  %11 = add nsw i32 undef, 1, !dbg !30, !verifier.code !15
-  call void @llvm.dbg.value(metadata i32 %11, metadata !31, metadata !DIExpression()), !dbg !14, !verifier.code !15
-  ret i32 0, !dbg !32, !verifier.code !15
+  call void @llvm.dbg.value(metadata i32* null, metadata !13, metadata !DIExpression()), !dbg !14, !verifier.code !15
+  %1 = call noalias i8* @malloc(i64 4) #3, !dbg !16, !verifier.code !15
+  %2 = bitcast i8* %1 to i32*, !dbg !17, !verifier.code !15
+  call void @llvm.dbg.value(metadata i32* %2, metadata !13, metadata !DIExpression()), !dbg !14, !verifier.code !15
+  call void @llvm.dbg.value(metadata i32* null, metadata !13, metadata !DIExpression()), !dbg !14, !verifier.code !15
+  call void @llvm.dbg.value(metadata i32 10, metadata !18, metadata !DIExpression()), !dbg !14, !verifier.code !15
+  %3 = load i32, i32* null, align 4, !dbg !19, !verifier.code !15
+  call void @llvm.dbg.value(metadata i32 %3, metadata !18, metadata !DIExpression()), !dbg !14, !verifier.code !15
+  ret i32 0, !dbg !20, !verifier.code !15
 }
 
 ; Function Attrs: nounwind readnone speculatable willreturn
@@ -30,9 +21,6 @@ declare void @llvm.dbg.declare(metadata, metadata, metadata) #1
 
 ; Function Attrs: nounwind
 declare dso_local noalias i8* @malloc(i64) #2
-
-; Function Attrs: nounwind
-declare dso_local void @free(i8*) #2
 
 ; Function Attrs: nounwind readnone speculatable willreturn
 declare void @llvm.dbg.value(metadata, metadata, metadata) #1
@@ -61,26 +49,14 @@ attributes #3 = { nounwind }
 !7 = !{i32 7, !"Dwarf Version", i32 4}
 !8 = !{i32 2, !"Debug Info Version", i32 3}
 !9 = !{i32 1, !"wchar_size", i32 4}
-!10 = distinct !DISubprogram(name: "main", scope: !1, file: !1, line: 153, type: !11, scopeLine: 153, spFlags: DISPFlagDefinition, unit: !0, retainedNodes: !2)
+!10 = distinct !DISubprogram(name: "main", scope: !1, file: !1, line: 3, type: !11, scopeLine: 3, spFlags: DISPFlagDefinition, unit: !0, retainedNodes: !2)
 !11 = !DISubroutineType(types: !12)
 !12 = !{!5}
-!13 = !DILocalVariable(name: "num", scope: !10, file: !1, line: 156, type: !5)
+!13 = !DILocalVariable(name: "i", scope: !10, file: !1, line: 4, type: !4)
 !14 = !DILocation(line: 0, scope: !10)
 !15 = !{i1 false}
-!16 = !DILocation(line: 157, column: 31, scope: !10)
-!17 = !DILocation(line: 157, column: 34, scope: !10)
-!18 = !DILocation(line: 157, column: 24, scope: !10)
-!19 = !DILocation(line: 157, column: 18, scope: !10)
-!20 = !DILocalVariable(name: "j", scope: !10, file: !1, line: 157, type: !4)
-!21 = !DILocation(line: 158, column: 22, scope: !10)
-!22 = !DILocation(line: 158, column: 12, scope: !10)
-!23 = !DILocation(line: 158, column: 16, scope: !10)
-!24 = !DILocation(line: 159, column: 23, scope: !10)
-!25 = !DILocation(line: 159, column: 20, scope: !10)
-!26 = !DILocation(line: 159, column: 27, scope: !10)
-!27 = !DILocalVariable(name: "nnum", scope: !10, file: !1, line: 159, type: !5)
-!28 = !DILocation(line: 160, column: 14, scope: !10)
-!29 = !DILocation(line: 160, column: 9, scope: !10)
-!30 = !DILocation(line: 161, column: 10, scope: !10)
-!31 = !DILocalVariable(name: "i", scope: !10, file: !1, line: 154, type: !5)
-!32 = !DILocation(line: 163, column: 5, scope: !10)
+!16 = !DILocation(line: 5, column: 16, scope: !10)
+!17 = !DILocation(line: 5, column: 9, scope: !10)
+!18 = !DILocalVariable(name: "j", scope: !10, file: !1, line: 7, type: !5)
+!19 = !DILocation(line: 8, column: 9, scope: !10)
+!20 = !DILocation(line: 10, column: 5, scope: !10)
