testcases/printtest/exec.bpl
@@ -6,49 +6,20 @@ axiom (main == $sub.ref(0, 1032));
 procedure {:entrypoint} main()
   returns ($r: i32)
 {
-  var $i0: i64;
-  var $i1: i64;
-  var $p2: ref8;
-  var $p3: ref32;
-  var $i4: i32;
-  var $p5: ref32;
-  var $p6: ref32;
-  var $i7: i32;
-  var $i8: i32;
-  var $p9: ref8;
-  var $i10: i32;
+  var $p0: ref8;
+  var $p1: ref32;
+  var $i2: i32;
 $bb0:
-  assume {:sourceloc "../testcases/printtest/exec.c", 157, 31} true;
+  assume {:sourceloc "../testcases/printtest/exec.c", 5, 16} true;
   call {:cexpr "smack:entry:main"} boogie_si_record_ref(main);
-  assume {:sourceloc "../testcases/printtest/exec.c", 157, 31} true;
-  $i0 := $sext.i32.i64(5);
-  assume {:sourceloc "../testcases/printtest/exec.c", 157, 34} true;
-  $i1 := $mul.i64($i0, 4);
-  assume {:sourceloc "../testcases/printtest/exec.c", 157, 24} true;
-  call $p2 := malloc($i1);
-  assume {:sourceloc "../testcases/printtest/exec.c", 157, 18} true;
-  $p3 := $bitcast.ref.ref($p2);
-  assume {:sourceloc "../testcases/printtest/exec.c", 158, 22} true;
-  $i4 := $add.i32(5, $sub.i32(0, 1));
-  assume {:sourceloc "../testcases/printtest/exec.c", 158, 12} true;
-  $p5 := $add.ref($p3, $mul.ref(1, 4));
-  assume {:sourceloc "../testcases/printtest/exec.c", 158, 16} true;
-  $M.0 := $store.i32($M.0, $p5, $i4);
-  assume {:sourceloc "../testcases/printtest/exec.c", 159, 23} true;
-  $p6 := $add.ref($p3, $mul.ref(1, 4));
-  assume {:sourceloc "../testcases/printtest/exec.c", 159, 20} true;
-  $i7 := $load.i32($M.0, $p6);
-  assume {:sourceloc "../testcases/printtest/exec.c", 159, 27} true;
-  $i8 := $add.i32($i7, $sub.i32(0, 1));
-  call {:cexpr "nnum"} boogie_si_record_i32($i8);
-  assume {:sourceloc "../testcases/printtest/exec.c", 160, 14} true;
-  $p9 := $bitcast.ref.ref($p3);
-  assume {:sourceloc "../testcases/printtest/exec.c", 160, 9} true;
-  call free_($p9);
-  assume {:sourceloc "../testcases/printtest/exec.c", 161, 10} true;
-  $i10 := $add.i32($u0, 1);
-  call {:cexpr "i"} boogie_si_record_i32($i10);
-  assume {:sourceloc "../testcases/printtest/exec.c", 163, 5} true;
+  assume {:sourceloc "../testcases/printtest/exec.c", 5, 16} true;
+  call $p0 := malloc(4);
+  assume {:sourceloc "../testcases/printtest/exec.c", 5, 9} true;
+  $p1 := $bitcast.ref.ref($p0);
+  assume {:sourceloc "../testcases/printtest/exec.c", 8, 9} true;
+  $i2 := $load.i32($M.0, $0.ref);
+  call {:cexpr "j"} boogie_si_record_i32($i2);
+  assume {:sourceloc "../testcases/printtest/exec.c", 10, 5} true;
   $r := 0;
   return;
 }
@@ -62,23 +33,16 @@ procedure  malloc($i0: i64)
 {
   call $r := $malloc($i0);
 }
-const free_: ref;
-axiom (free_ == $sub.ref(0, 4128));
-procedure  free_($p0: ref)
-{
-  call $free($p0);
-}
 const llvm.dbg.value: ref;
-axiom (llvm.dbg.value == $sub.ref(0, 5160));
+axiom (llvm.dbg.value == $sub.ref(0, 4128));
 procedure  llvm.dbg.value($p0: ref, $p1: ref, $p2: ref);
 const __SMACK_static_init: ref;
-axiom (__SMACK_static_init == $sub.ref(0, 6192));
+axiom (__SMACK_static_init == $sub.ref(0, 5160));
 procedure  __SMACK_static_init()
 {
 $bb0:
   return;
 }
-const {:global_variable} $u0: i32;
 procedure  boogie_si_record_i32(x: i32);
 procedure  boogie_si_record_ref(x: ref);
 procedure  $initialize()
